pcuic/theories/PCUICClosed.v
@@ -355,14 +355,13 @@ Proof.
     unfold test_def. simpl. toProp.
     split.
     rewrite -> app_context_length in *. rewrite -> Nat.add_comm in *.
-    eapply closedn_lift_inv in H1; eauto. lia.
-    subst types.
-    now rewrite -> app_context_length, fix_context_length in H0.
-    eapply (nth_error_all) in H; eauto. simpl in *.
+    eapply closedn_lift_inv in H2; eauto. lia.
+    now rewrite -> app_context_length, fix_context_length in H1.
+    eapply (nth_error_all) in H0; eauto. simpl in *.
     intuition. toProp.
-    subst types. rewrite app_context_length in H0.
-    rewrite Nat.add_comm in H0.
-    now eapply closedn_lift_inv in H0.
+    rewrite app_context_length in H1.
+    rewrite Nat.add_comm in H1.
+    now eapply closedn_lift_inv in H1.
 
   - destruct X2; intuition eauto.
     + destruct i as [[u [ctx [Heq Hi]]] Hwfi]. simpl in Hwfi.
